\documentclass[11pt]{article}

\usepackage[cp1251]{inputenc}
\usepackage[english]{babel}
\usepackage{amsmath}
\usepackage{amsthm}
\usepackage{amsfonts}
\usepackage{amssymb}
\usepackage{verbatim}
\usepackage[T1]{fontenc}
\usepackage{hyperref}
\usepackage{enumerate}


\DeclareMathOperator{\supp}{supp}
\DeclareMathOperator{\roots}{roots}
\DeclareMathOperator{\AG}{AG}
\DeclareMathOperator{\G}{G}
\DeclareMathOperator{\avg}{avg}

\newcommand{\R}{\mathbb{R}}
\newcommand{\e}{\varepsilon}

\newtheorem{theorem}{Theorem}[section]
\newtheorem{lemma}[theorem]{Lemma}
\newtheorem{proposition}[theorem]{Proposition}
\newtheorem{corollary}[theorem]{Corollary}
\newtheorem{definition}[theorem]{Definition}


\begin{document}
\begin{center}
\textbf{On the average root gap size after applying $(1-D)$ operator}\\
Stanislav Atanasov and Christopher Shriver
\end{center}

An operator ...
Throughout the paper, we use $\lambda_{min}=\lambda_1\leq \cdots \leq \lambda_n = \lambda_{max}$ to denote the roots of the real rooted polynomial $P(x)$. Of particular interest for us are the \emph{average gap}, $\AG(P)$, of the polynomial $P(x)$, defined by $\AG(P)=\frac{\lambda_{max} - \lambda_{min}}{\deg P - 1}$, as well as the \emph{$i$-th partial gap} $G_i(P)$, given by $\lambda_{max}-\lambda_i$. We establish the following

\begin{theorem}
please fill the exact formula
\end{theorem}

\subsection{Average gap after many iterations}
 In this section, we show that the average gap approaches infinity when we apply the $(1-D)$ operator many times. More precisely, for any sequence of real-rooted polynomials $\{f_k\}_1^{\infty}$ satisfying $f_{k+1}(x) = (1-D)^k f_{1}(x),$ it holds that $\lim_{n\to \infty} \AG(f_n) = \infty$. We prove this claim in two short steps.

 \begin{lemma}
 \label{degree two avg distance}
 Let $f(x)$ be a real-rooted quadratic polynomial with roots $\lambda_1 \leq \lambda_2$. Then $\AG((1-D)^n f) \to +\infty$ as ${n\to \infty}$.
 \end{lemma}
\proof
Without loss of generality, we might assume that $f(x)$ is monic and write it as $x^2+ax+b$. The Vieta's formulas yield $\AG(f) = \lambda_2 - \lambda_1 = \sqrt{a^2 - 4b}$. Introduce the sequence $\{f_k\}_{0}^\infty$ of polynomials given by $f_{k} (x)= (1-D)^k f_0(x)$ and $f_0(x) = f(x)$. Since $(1-D)$ preserves real-rootedness all $f_k(x)$ are real-rooted. In similar fashion, denote $\lambda_1^{(k)} \leq \lambda_2^{(k)}$ to be the two real roots of $f_k(x)$. Using Vieta's formulas once again, we obtain
 \[\AG(f_k) = \sqrt{\AG(f_{k-1})^2 + 4}.~(*)\]

 Clearly, $\AG(f_k) > \AG(f_{k-1})$ for every $k\ge 1$ and so  $\lim \AG(f_k)$ exists (possibly, and as we shall see, infinite). Assume it is finite, say $l$. Taking the limit on both sides of $(*)$ leads to $l = \sqrt{l^2 + 4},$ which is evidently impossible. Hence, $\lim \AG(f_k) = \infty$. \qed

\begin{lemma}
\label{degree two - slowest movement}
Let $f(x)$ be a real-rooted polynomial with roots $\lambda_{min}=\lambda_1 < \lambda_2 \cdots \leq \lambda_{n-1} < \lambda_n = \lambda_{max}$. Then $(n-1) \cdot AG\big[(1-D)f\big] \geq AG\big[(1-D)f_{1,n}\big]$, where $f_{1,n} = (x - \lambda_{min})(x - \lambda_{max})$ is the quadratic polynomial with roots $\lambda_1$ and $\lambda_n$.
\end{lemma}
\proof Note that since $\lambda_{min}$ and $\lambda_{max}$ are simple roots, they are not roots of $(1-D)f$. Thus, the biggest and smallest root of $(1-D)f$ are the biggest and smallest root of $\frac{(1-D)f}{f}$. Let $x_0\in\mathbb{R}$ be the biggest root of $(1-D)f(x)$. By the above remark, we have
\[\frac{(1-D)f}{f}(x_0) = 0 \Leftrightarrow \sum_{i=1}^n \frac{1}{x_0 - \lambda_i} = 1.\]

Note that $x_0 > \lambda_i,~\forall 1\leq i \leq n$ and so $\frac{1}{x_0 - \lambda_1} + \frac{1}{x_0 - \lambda_n} < \sum_{i=1}^n \frac{1}{x_0 - \lambda_i} = 1.$ In particular, since $\frac{(1-D)f_{1,n}}{f_{1,n}}(x) = \frac{1}{x - \lambda_1} + \frac{1}{x - \lambda_n}$ is monotonically decreasing on $(\lambda_n, +\infty)$, the above inequality implies that the biggest root of $(1-D)f_{1,n}$ is smaller than $x_0$. Similarly, we prove that the smallest root of $(1-D)f_{1,n}$ is bigger than the smallest root of $(1-D)f$. Hence, the claim follows. \qed

Now, combining the two lemmata, we easily derive

\begin{proposition}For any sequence of real-rooted polynomials $\{f_k\}_0^{\infty}$ satisfying $f_{k}(x) = (1-D)^k f_{0}(x),$ we have $\lim_{n\to \infty} \AG(f_n) =  \infty.$
\end{proposition}
\label{avg gap goes to infty}
\proof Note that if $\lambda$ is a root of multiplicity $k$, then it is a root of multiplicity $k-1$ of $(1-D)f$. Therefore, after $\deg f$ applications of the $(1-D)$ operator, we obtain a polynomial with simple roots. Therefore we might, without loss of generality, assume that $f_0$ has simple roots. Otherwise, we could just pick $f_{\deg f_0}$ as a first element of our sequence. Suppose $\lambda_{min}=\lambda_1 < \lambda_2 \cdots \leq \lambda_{n-1} < \lambda_n = \lambda_{max}$ are the roots of $f_0(x)$. Now repeated application of Lemma~\ref{degree two - slowest movement}, coupled with the observation that $\AG((1-D)[(x-a)(x-b)]) \geq \AG((1-D)[(x-c)(x-d)])$ whenever $|a-b|\geq|c-d|$, leads to

\[\AG(f_k)= \AG((1-D)^kf_0)\geq\AG((1-D)^k [(x-\lambda_{min})(x-\lambda_{max})]),\]
for every $k\in\mathbb{N}$. Applying Lemma~\ref{degree two avg distance} shows that, as $k$ grows, the right hand side goes to $\infty$, and thus so does the expression on the left. \qed

\subsection{The growth of $i$-th partial gap}
In the previous section, we concluded that the average gap increases without bound upon repeated applications of the $(1-D)$ operator. Recall that the $i$-th partial gap of a polynomial $f$ is $G_i = \lambda_{max} - \lambda_{n-i}$. Proposition~\ref{avg gap goes to infty} asserts that the $n$-th partial gap, i.e. a multiple of the average gap, goes to infinity. A natural question is to ask whether the same thing holds for each of the partial gaps. As we shall see, this is indeed true.

\begin{comment}
\begin{lemma}
\label{all gaps grow - case with 3}
Let $f(x)$ be a real-rooted cubic polynomial with roots $\lambda_1 \leq \lambda_2 \leq \lambda_3$. Construct a sequence $\{f_k\}_1^\infty$ defined by $f_k(x) = (1-D)^k f_0(x)$, where $f_0(x) = f(x)$. Then we have that
\[\lim_{n\to \infty} G_1 (f_n) = \infty\]
\end{lemma}
\proof
As discussed earlier, we might without loss of generality assume that all roots of $f(x)$ are simple. By Proposition~\ref{avg gap goes to infty}, we establish that $\AG(f_k)$ goes to $\infty$. In particular, if we denote by $\lambda^{(k)}_1 < \lambda^{(k)}_2 < \lambda^{(k)}_3$ the roots of $f_k(x)$, we have $\underbrace{|\lambda^{(k)}_3 - \lambda^{(k)}_2|}_{\alpha_k} + \underbrace{|\lambda^{(k)}_2 - \lambda^{(k)}_1}_{\beta_k}|$ grows to infinity.

As discussed earlier, we might without loss of generality assume that all roots of $f(x)$ are simple. By Proposition~\ref{avg gap goes to infty}, we establish that $\AG(f_k)$ goes to $\infty$. In particular, if we denote by $\lambda^(k)_1 < \lambda^{(k)}_2 < \lambda^{(k)}_3$ the roots of $f_k(x)$, we have $\underbrace{|\lambda^{(k)}_3 - \lambda^{(k)}_2|}_{\alpha_k} + \underbrace{|\lambda^{(k)}_2 - \lambda^{(k)}_1}_{\beta_k}|$ grows to infinity. This implies that for big enough $k$ one of the numbers $\alpha_k$ or $\beta_k$ is arbitrarily big.

\textbf{1 case:} Suppose there exist $N$ such that $\alpha_n > \beta_n$ and $\beta_n > \alpha_n$ holds for every $n\geq N$. Assume the later holds. Then since $\alpha_n + \beta_n = \AG(f_n)$, we derive that $\beta_ n > \frac{\AG(f_n)}{2},~\forall n \geq N$. Since the right hand side goes to infinity, then so does the right hand side, which is what we wanted to prove. For the sake of contradiction, assume that $\alpha_n > \beta_n,~\forall n \geq N$. Then for any $n$, we have for any of the roots of $f_{n+1}(x) = (1-D)f_n(x)$ that
\[\frac{1}{x_0 - \lambda^{(n)}_1} + \frac{1}{x_0 - \lambda^{(n)}_2} + \frac{1}{x_0 - \lambda^{(n)}_3} = 1\]
Let $\varepsilon > 0$. By assumption there exist $N$ so that for any $n \geq N$ the two bigger roots of $f_{n+1}(x)$ are far enough from $\lambda^{(n)}_1$ so that $\frac{1}{x_0 - \lambda^{(n)}_1} < \varepsilon$, implying $\frac{1}{x_0 - \lambda^{(n)}_2} + \frac{1}{x_0 - \lambda^{(n)}_3} < 1 - \varepsilon$. Since $\frac{1}{x - \lambda^{(n)}_2} + \frac{1}{x - \lambda^{(n)}_3}$ is monotonically decreasing function, the distance $|\mu_2 - \mu_1|$ between the roots $\mu_1 < \mu_2$ of $g(x) = \frac{1}{x - \lambda^{(n)}_2} + \frac{1}{x - \lambda^{(n)}_3} - 1 + \varepsilon = 0$ is smaller than the distance $|\lambda^{(n+1)}_3 - \lambda^{(n+1)}_2|$. By Vieta's formula we then establish

\[|\lambda^{(n+1)}_3 - \lambda^{(n+1)}_2|\ge |\mu_2 - \mu_1| = \sqrt{|\lambda^{(n)}_3 - \lambda^{(n)}_2|^2 + \frac{4}{(1+\varepsilon)^2}} > \sqrt{|\lambda^{(n)}_3 - \lambda^{(n)}_2|^2 +4}.\]
Clearly, this implies that $|\lambda^{(N + k)}_3 - \lambda^{(N+k)}_2|$ is monotonically increasing sequence. Assuming it has a finite limit $l$, leads to $l > \sqrt{l^2 +4}$, which is absurd. Hence, $\lim_{n\to \infty} |\lambda^{(n)}_3 - \lambda^{(n)}_2|=\lim_{k\to \infty} |\lambda^{(N + k)}_3 - \lambda^{(N+k)}_2| = \infty,$ as claimed.

\textbf{2 case:}
Suppose now that for every $M$, there exist $m, k > M$ such that $\alpha_n > \beta_n$ and $\beta_k > \alpha_k$. Let $l$ be an index for "transition", i.e. $\alpha_l > \beta_l$ and $\beta_{l+1} > \alpha_{l+1}$ or vice versa. Without loss of generality, we are in the first situation. Recall that the $(1-D)$ operator moves $\lambda^{(l)}_{1}$ to the right by at most 1, $\lambda^{(l)}_{2}$ - by at most 2, and $\lambda^{(l)}_{3}$ - by at most 3. Therefore, $\alpha_{l+1} > \alpha_l - 1$ and $\beta_{l+1} < \beta_l + 3$. Combining these two inequalities with $\alpha_l > \beta_l$ and $\beta_{l+1} > \alpha_{l+1}$ leads to $\beta_l > \frac{\AG(f_l)}{2} - 2$. Since $l$ can be arbitrarily big, so can be $\AG(f_l)$. Due to Lemma~\ref{minimal gap increases}, this implies that the minimal gap between roots goes unbounded. In particular, $\lim \alpha_n = \lim \beta_n = \infty$.
\qed
\end{comment}


Now, let us analyse the actual gaps between the roots. For that reason introduce $d_{i+1}(f(x)) := \lambda_{i+1}(f(x)) - \lambda_i(f(x))$.

\begin{proposition}
\label{minimal gap is unbounded}
Suppose there is a sequence $\{f_k\}_1^\infty$ of real-rooted polynomials defined by $f_k(x) = (1-D)^k f_0(x)$, where $f_0(x)$ is real-rooted of degree $m$. Then
\[\lim_{n\to\infty} \min_{1\leq i \leq m} d_i (f_n) = \infty\]
holds true.
\end{proposition}
\proof Note first that Lemma~\ref{minimal gap increases} asserts the existence of such a limit. For the sake of contradiction, assume it is finite, say $l$.

We first analyze the behavior of the gaps between nonconsecutive roots of the $f_k(x)$ as $k$ increases. Applying Lemma~\ref{degree two avg distance} in combination with Lemma~\ref{degree two - slowest movement} easily show that all such gaps increase unboundedly and go to infinity. In particular, we have that
\[|\lambda^{(n)}_{i+2} - \lambda^{(n)}_i|\to \infty\text{~as~$n\to\infty$}\]
for every $1\leq i \leq n-2$.

Pick arbitrarily large number $L\in\mathbb{R}$ and some $\varepsilon > 0$. Then there exist a big enough $M$ so that for all $n\geq M$ we have that all double gaps satisfy $|\lambda^{(n)}_{i+2} - \lambda^{(n)}_i| > L + l$ and also $\min_{1\leq i \leq m} d_i (f_n)> l - \varepsilon$. Denote by $\{j_k\}_{n}^{\infty}$ the sequence of indexes such that $d_{j_n}:=\min_{1\leq i \leq m} d_i (f_n)$ for $n\geq M$. Since both distances $|\lambda^{(n)}_{j_n+1} - \lambda^{(n)}_{j_n-1}|$ and $|\lambda^{(n)}_{j_n+2} - \lambda^{(n)}_{j_n}|$ are bigger than $L + l$, we have that $d_{j_n-1}> L$ and $d_{j_n+1} > L$ for all $n\geq M$.

Note that $x_0 > \lambda_i,~\forall 1\leq i \leq n$ and so $\frac{1}{x_0 - \lambda_1} + \frac{1}{x_0 - \lambda_n} < \sum_{i=1}^n \frac{1}{x_0 - \lambda_i} = 1.$ In particular, since $\frac{(1-D)f_{1,n}}{f_{1,n}}(x) = \frac{1}{x - \lambda_1} + \frac{1}{x - \lambda_n}$ is monotonically decreasing function on $(\lambda_n, +\infty)$, the above inequality implies that the biggest root of $(1-D)f_{1,n}$ is smaller than $x_0$. Similarly, we prove that the smallest root of $(1-D)f_{1,n}$ is bigger than the smallest root of $(1-D)f$. Hence, the claim follows. \qed

Now, combining the two lemmata, we easily derive

\begin{proposition}For any sequence of real-rooted polynomials $\{f_k\}_0^{\infty}$, satisfying $f_{k+1}(x) = (1-D)^k f_{0}(x),$ we have $\lim_{n\to \infty} \AG(f_n) =  \infty.$
\end{proposition}
\label{avg gap goes to infty}
\proof Note that if $\lambda$ is a root of multiplicity $k$, then it is a root of multiplicity $k-1$ of $(1-D)f$. Therefore, after $deg f$ applications of the $(1-D)$ operator, we obtain a polynomial with simple roots. Therefore, we might, without loss of generality, assume that $f_0$ has simple roots. Otherwise, we could just pick $f_{deg f_0}$ as a first element of our sequence. Suppose $\lambda_{min}=\lambda_1 < \lambda_2 \cdots \leq \lambda_{n-1} < \lambda_n = \lambda_{max}$ are the roots of $f_0(x)$. Now repeated application of Lemma~\ref{degree two - slowest movement}, coupled with the observation that $\AG((1-D)[(x-a)(x-b)]) \geq \AG((1-D)[(x-c)(x-d)])$ whenever $c < a,~b<d$, leads to

\[\AG(f_k)= \AG((1-D)^kf_0)\geq\AG((1-D)^k [(x-\lambda_{min})(x-\lambda_{max})]),\]
for every $k\in\mathbb{N}$. Applying Lemma~\ref{degree two avg distance} shows that, as $k$ grows, the right hand side goes to $\infty$, and thus so does the expression on the left. \qed

\subsection{The growth of $i$-th partial gap}
In the previous section, we concluded that the average gap increases without bound upon repeated applications of the $(1-D)$ operator. Recall, that $i$-th partial gap of a polynomial $f$ is $G_i = \lambda_{max} - \lambda_{n-i}$. Proposition~\ref{avg gap goes to infty} asserts that the $n$-th partial gap, i.e. a multiple of the average gap, goes to infinity. A natural question is to ask whether the same thing holds for each of the partial gaps. As we shall see, this is indeed true.

\begin{lemma}
\label{minimal gap increases}
 Consider sequence of real-rooted polynomials $\{f_k\}_1^\infty$ given by $f_k(x) = (1-D)^k f_0(x)$. Then
 \[\min |\lambda^{(n+1)}_{i+1} - \lambda^{(n+1)}_i | \geq \min |\lambda^{(n)}_{i+1} - \lambda^{(n)}_i |\]
\end{lemma}
\proof (From \cite{diffspacing}, attributed there to M. Riesz) Let $f$ be a polynomial with roots $\lambda_1\leq\cdots\leq\lambda_n$, and let $g = (1-D)f$. If $f$ has a multiple root, then $\min |\lambda_{i+1}-\lambda_i| = 0$ so the Lemma is true. Suppose instead that all roots of $f$ are simple. Then all roots of $g$ are roots of $\frac{(1-D)f}{f}$, and therefore solutions to the equation
 \[ \sum_{i=1}^n \frac{1}{x-\lambda_i} = 1. \]
Suppose $q<p$ are adjacent roots of $g$ that are closer together than any two roots of $f$, i.e.
 \[ p - q < \lambda_{i+1}-\lambda_i \quad \forall i. \]
This is equivalent to $p-\lambda_{i+1}<q-\lambda_i$, and since both sides are always the same sign we have
 \[ \frac{1}{p-\lambda_{i+1}} > \frac{1}{q-\lambda_i} \quad \forall i. \]
$p,q$ both being solutions to the above equation then implies
 \[ 0 = \sum_{i=1}^n \Big(\frac{1}{p-\lambda_i} - \frac{1}{q-\lambda_i}\Big) = \sum_{i=1}^{n-1}\Big(\frac{1}{p-\lambda_{i+1}} - \frac{1}{q-\lambda_i}\Big) + \frac{1}{p-\lambda_1} - \frac{1}{q-\lambda_n} > 0, \]
which is a contradiction. Therefore $p$ and $q$ must be at least as far apart as any pair of roots of $f$, and the lemma immediately follows.
\qed

\begin{comment}
\begin{lemma}
\label{all gaps grow - case with 3}
Let $f(x)$ be a real-rooted cubic polynomial with roots $\lambda_1 \leq \lambda_2 \leq \lambda_3$. Construct a sequence $\{f_k\}_1^\infty$ defined by $f_k(x) = (1-D)^k f_0(x)$, where $f_0(x) = f(x)$. Then we have that
\[\lim_{n\to \infty} G_1 (f_n) = \infty\]
\end{lemma}
\proof
As discussed earlier, we might without loss of generality assume that all roots of $f(x)$ are simple. By Proposition~\ref{avg gap goes to infty}, we establish that $\AG(f_k)$ goes to $\infty$. In particular, if we denote by $\lambda^{(k)}_1 < \lambda^{(k)}_2 < \lambda^{(k)}_3$ the roots of $f_k(x)$, we have $\underbrace{|\lambda^{(k)}_3 - \lambda^{(k)}_2|}_{\alpha_k} + \underbrace{|\lambda^{(k)}_2 - \lambda^{(k)}_1}_{\beta_k}|$ grows to infinity.

As discussed earlier, we might without loss of generality assume that all roots of $f(x)$ are simple. By Proposition~\ref{avg gap goes to infty}, we establish that $\AG(f_k)$ goes to $\infty$. In particular, if we denote by $\lambda^(k)_1 < \lambda^{(k)}_2 < \lambda^{(k)}_3$ the roots of $f_k(x)$, we have $\underbrace{|\lambda^{(k)}_3 - \lambda^{(k)}_2|}_{\alpha_k} + \underbrace{|\lambda^{(k)}_2 - \lambda^{(k)}_1}_{\beta_k}|$ grows to infinity. This implies that for big enough $k$ one of the numbers $\alpha_k$ or $\beta_k$ is arbitrarily big.

\textbf{1 case:} Suppose there exist $N$ such that $\alpha_n > \beta_n$ and $\beta_n > \alpha_n$ holds for every $n\geq N$. Assume the later holds. Then since $\alpha_n + \beta_n = \AG(f_n)$, we derive that $\beta_ n > \frac{\AG(f_n)}{2},~\forall n \geq N$. Since the right hand side goes to infinity, then so does the right hand side, which is what we wanted to prove. For the sake of contradiction, assume that $\alpha_n > \beta_n,~\forall n \geq N$. Then for any $n$, we have for any of the roots of $f_{n+1}(x) = (1-D)f_n(x)$ that
\[\frac{1}{x_0 - \lambda^{(n)}_1} + \frac{1}{x_0 - \lambda^{(n)}_2} + \frac{1}{x_0 - \lambda^{(n)}_3} = 1\]
Let $\varepsilon > 0$. By assumption there exist $N$ so that for any $n \geq N$ the two bigger roots of $f_{n+1}(x)$ are far enough from $\lambda^{(n)}_1$ so that $\frac{1}{x_0 - \lambda^{(n)}_1} < \varepsilon$, implying $\frac{1}{x_0 - \lambda^{(n)}_2} + \frac{1}{x_0 - \lambda^{(n)}_3} < 1 - \varepsilon$. Since $\frac{1}{x - \lambda^{(n)}_2} + \frac{1}{x - \lambda^{(n)}_3}$ is monotonically decreasing function, the distance $|\mu_2 - \mu_1|$ between the roots $\mu_1 < \mu_2$ of $g(x) = \frac{1}{x - \lambda^{(n)}_2} + \frac{1}{x - \lambda^{(n)}_3} - 1 + \varepsilon = 0$ is smaller than the distance $|\lambda^{(n+1)}_3 - \lambda^{(n+1)}_2|$. By Vieta's formula we then establish

\[|\lambda^{(n+1)}_3 - \lambda^{(n+1)}_2|\ge |\mu_2 - \mu_1| = \sqrt{|\lambda^{(n)}_3 - \lambda^{(n)}_2|^2 + \frac{4}{(1+\varepsilon)^2}} > \sqrt{|\lambda^{(n)}_3 - \lambda^{(n)}_2|^2 +4}.\]
Clearly, this implies that $|\lambda^{(N + k)}_3 - \lambda^{(N+k)}_2|$ is monotonically increasing sequence. Assuming it has a finite limit $l$, leads to $l > \sqrt{l^2 +4}$, which is absurd. Hence, $\lim_{n\to \infty} |\lambda^{(n)}_3 - \lambda^{(n)}_2|=\lim_{k\to \infty} |\lambda^{(N + k)}_3 - \lambda^{(N+k)}_2| = \infty,$ as claimed.

\textbf{2 case:}
Suppose now that for every $M$, there exist $m, k > M$ such that $\alpha_n > \beta_n$ and $\beta_k > \alpha_k$. Let $l$ be an index for "transition", i.e. $\alpha_l > \beta_l$ and $\beta_{l+1} > \alpha_{l+1}$ or vice versa. Without loss of generality, we are in the first situation. Recall that the $(1-D)$ operator moves $\lambda^{(l)}_{1}$ to the right by at most 1, $\lambda^{(l)}_{2}$ - by at most 2, and $\lambda^{(l)}_{3}$ - by at most 3. Therefore, $\alpha_{l+1} > \alpha_l - 1$ and $\beta_{l+1} < \beta_l + 3$. Combining these two inequalities with $\alpha_l > \beta_l$ and $\beta_{l+1} > \alpha_{l+1}$ leads to $\beta_l > \frac{\AG(f_l)}{2} - 2$. Since $l$ can be arbitrarily big, so can be $\AG(f_l)$. Due to Lemma~\ref{minimal gap increases}, this implies that the minimal gap between roots goes unbounded. In particular, $\lim \alpha_n = \lim \beta_n = \infty$.
\qed
\end{comment}

Now, let us analyse the actual gaps between the roots. For that reason introduce $d_{i+1}(f) := \lambda_{i+1}(f) - \lambda_i(f)$.

\begin{lemma}
\label{minimal gap shall approach}
 Consider a sequence $\{f_k\}_1^\infty$ of real-rooted polynomials defined by $f_k(x) = (1-D)^k f_0(x)$, where $f_0(x)$ is real-rooted of degree $m$. Suppose for some $n\in\mathbb{N}$, we have that there exists an index $1\leq i\leq n-1$ satisfying $d_{i-1} \geq L$ and $d_{i+1} \geq L$ for some real number $L$. Then we have that $\lambda^{(n+1)}_i$ is smaller than the smaller root of
 \[\frac{i-1}{L}+\frac{1}{x-\lambda^{(n)}_i} + \frac{1}{x-\lambda^{(n)}_{i+1}} = 1.\]
 Similarly, $\lambda^{(n+1)}_{i+1}$ is bounded from below by the bigger root of 
 \[\frac{n-(i+1)}{L}+\frac{1}{x-\lambda^{(n)}_i} + \frac{1}{x-\lambda^{(n)}_{i+1}} = 1.\]
\end{lemma}
\proof
We only need to show the first bound since the second one can be proven analogously. We know that $\lambda^{(n+1)}_i\in(\lambda^{(n)}_i,\lambda^{(n)}_{i+1})$. Then the claim follows since for every $x\in (\lambda^{(n)}_i,\lambda^{(n)}_{i+1})$ we have that
\[\sum^{i-1}_{k=1} \frac{1}{x-\lambda^{(n)}_k} + \frac{1}{x-\lambda^{(n)}_i} + \frac{1}{x-\lambda^{(n)}_{i+1}} + \sum^n_{k = i+2} \frac{1}{x-\lambda^{(n)}_k} < \frac{i-1}{L}+\frac{1}{x-\lambda^{(n)}_i} + \frac{1}{x-\lambda^{(n)}_{i+1}} \]
and that $\frac{1}{x-\lambda^{(n)}_i} + \frac{1}{x-\lambda^{(n)}_{i+1}}$ is monotonically decreasing in $(\lambda^{(n)}_i,\lambda^{(n)}_{i+1})$.
\qed


\begin{proposition}
\label{minimal gap is unbounded}
Suppose there is a sequence $\{f_k\}_1^\infty$ of real-rooted polynomials defined by $f_k(x) = (1-D)^k f_0(x)$, where $f_0(x)$ is real-rooted of degree $m$. Then
\[\lim_{n\to\infty} \min_{1\leq i \leq m} d_i (f_n) = \infty\]
holds true.
\end{proposition}
\proof Lemma~\ref{minimal gap increases} asserts the existence of such a limit. For the sake of contradiction, assume it is finite, say $l$.

We first analyze the behavior of the gaps between nonconsecutive roots of the $f_k(x)$ as $k$ increases. Applying Lemma~\ref{degree two avg distance} in combination with Lemma~\ref{degree two - slowest movement} easily show that all such gaps increase unboundedly and go to infinity. In particular, we have that
\[|\lambda^{(n)}_{i+2} - \lambda^{(n)}_i|\to \infty\text{~as~$n\to\infty$}\]
for every $1\leq i \leq n-2$.

Pick an arbitrarily large number $L\in\mathbb{R}$ and some $\varepsilon > 0$. Then there exist a big enough $M$ so that for all $n\geq M$ we have that all double gaps satisfy $|\lambda^{(n)}_{i+2} - \lambda^{(n)}_i| > L + l$ and also $\min_{1\leq i \leq m} d_i (f_n)> l - \varepsilon$. Denote by $\{j_k\}_{n}^{\infty}$ the sequence of indexes such that $d_{j_n}=\min_{1\leq i \leq m} d_i (f_n)$ for $n\geq M$. Since both distances $|\lambda^{(n)}_{j_n+1} - \lambda^{(n)}_{j_n-1}|$ and $|\lambda^{(n)}_{j_n+2} - \lambda^{(n)}_{j_n}|$ are bigger than $L + l$, we have that $d_{j_n-1}> L$ and $d_{j_n+1} > L$ for all $n\geq M$. 

This means that we are in the conditions of Lemma~\ref{minimal gap shall approach}, which gives us a lower bound of the $d_{j_{n+1}}$ for every $n\geq M$. However, note that if $L$ is big enough, the quantities $\frac{i-1}{L}$ and $\frac{n-(i+1)}{L}$ from Lemma~\ref{minimal gap shall approach} become negligibly small. Therefore, by continuity, for every $\delta > 0$, there is $M$ such that the corresponding $L$ is big enough such that the roots $\lambda^{(n+1)}_{j_n}$ and $\lambda^{(n+1)}_{j_n}$ are both within $\frac{\delta}{2}$ of the roots $\mu^{(n)}_1,~\mu^{(n)}_2$ of $\frac{1}{x-\lambda^{(n)}_{j_n}} + \frac{1}{x-\lambda^{(n)}_{j_n+1}} = 1,~\forall n\geq M$. In particular, $|\lambda^{(n+1)}_{j_n+1} - \lambda^{(n+1)}_{j_n}|>|\mu^{(n)}_1 - \mu^{(n)}_2| - \delta,~\forall n\geq M$.

Recall that $|\mu^{(n)}_1 - \mu^{(n)}_2|= \sqrt{|\lambda^{(n)}_{j_n+1} - \lambda^{(n)}_{j_n}|^2 + 4}$. Now, since $\varepsilon > 0$ was picked arbitrarily, we might assume it is small enough so that $\sqrt{|\lambda^{(n)}_{j_n+1} - \lambda^{(n)}_{j_n}|^2 + 4} > l$. Now, the choice of $\delta$ was independent of $\varepsilon$, so we pick $0< \delta <\sqrt{|\lambda^{(n)}_{j_n+1} - \lambda^{(n)}_{j_n}|^2 + 4} - |\mu^{(n)}_1 - \mu^{(n)}_2|$. This evidently leads to contradiction, which was based on the assumption that the limit $l$ is finite. Hence, $\lim_{n\to\infty} \min_{1\leq i \leq m} d_i (f_n) = \infty$, as desired. \qed

\subsection{Some additions/comments}
First, another lemma that I think can be useful elsewhere as well:
\begin{lemma}
	Suppose $f$ is a polynomial whose $i$th smallest root $\mu_i$ is moved (necessarily to the right) a distance $\delta$ by the $1-D$ operator. Given $\mu \in \R$, consider the polynomial $\tilde{f} = (x-\mu)f$. Then
	\begin{enumerate}
		\item if $\mu \leq \mu_i$, then $\lambda_{i+1}\big[(1-D)\tilde{f}\big] \geq \mu_i + \delta$ (note that since a root has been added to the left, the $(i+1)$th root of $\tilde{f}$ is the root which intuitively corresponds to the $i$th root of $f$), and 
		\item if $\mu > \mu_i$, then $\lambda_{i}\big[(1-D)\tilde{f}\big] \leq \mu_i + \delta$.
	\end{enumerate}
	Loosely speaking, the added root has the effect of `repelling' the old roots of $(1-D)f$.
\end{lemma}
\begin{proof}
	First consider the second case, $\mu > \mu_i$. If $\mu \leq \mu_i + \delta$, then the result follows immediately from interlacing. \\
	If instead $\mu > \mu_i + \delta$, we can use the logarithmic derivative to get the bound we want. If $\delta=0$ then $\mu_i$ is a root of multiplicity and adding the root $\mu$ will not change how much it moves. Assume instead then that $\delta>0$. Then $\mu_i+\delta$ is a root of $\frac{f^\prime}{f}$, i.e.
		\[ \sum_{j=1}^n \frac{1}{(\mu_i+\delta)-\mu_j} = 1. \]
	We would like to find the root of $(1-D)\tilde{f}$, that is the solution of
		\[ \sum_{j=1}^n \frac{1}{x-\mu_j} + \frac{1}{x-\mu} = 1, \]
	that is closest to the right of $\mu_i$. We know that for $x=\mu_i+\delta$ the sum is equal to 1 and the second term is negative, so the left hand side is less than 1. It is also apparent that the sum is much greater than 1 for $x$ just to the right of $\mu_i$, and continuous for $x \in (\mu_i, \mu_i+\delta)$. Therefore by the intermediate value theorem there is a solution in $(\mu_i, \mu_i+\delta)$ and the result immediately follows. \\
	The proof for $\mu<\mu_i$ is essentially the same.
\end{proof}

The following lemma easily follows:

\begin{lemma}
	Appending a root between two (not necessarily adjacent) roots increases the change in their difference upon applying $1-D$.
\end{lemma}
For example, if the gap between the roots of $(x-1)(x-3)$ changes by $\delta$, then the gap between the outer two roots of $(x-1)(x-2)(x-3)$ will change by more than $\delta$.

We already know that the gap between the largest and smallest roots is nondecreasing. The previous lemma can be used to show that it approaches infinity:

\begin{lemma}
\label{lem:maxgapinf}
	For any polynomial $f$,
	 \[ \lim_{n\to\infty} \lambda_{\max}\big[(1-D)^n f\big]-\lambda_{\min}\big[(1-D)^n f\big] = \infty. \]
\end{lemma}
\begin{proof}
	Because the quantity of interest is nondecreasing, it is enough to show that it has no finite limit. Suppose it did approach some number $l < \infty$. Then there is some number of iterations of $1-D$ after which the difference between the maximum and minimum roots is arbitrarily close to $l$. Suppose a polynomial with only two roots separated by $l$ has its gap increased by $\delta$. Then if the two roots are closer than $l$ and more roots are appended in between, the gap will still increase by at least $\delta$. Therefore if the gap between extremal roots is at least $l - \delta/2$, then after applying $1-D$ it will be at least $l + \delta/2$. This is a contradiction, so it must be that the gap is unbouded.
\end{proof}

Now we only need one more lemma, after which the theorem will follow by induction. First a definition: by `$n$-gap' we mean a gap between two roots that have $n-1$ other roots between them. For example $\mu_4-\mu_1$ is a 3-gap, and the difference between the minimum and maximum roots of a degree $m$ polynomial is an $(m-1)$-gap. Now the lemma:

\begin{lemma}
\label{lem:gapinduction}
	Suppose the $n$-gaps of a given polynomial approach infinity. Then the $n-1$ gaps do as well.
\end{lemma}
\begin{proof}
	Suppose the $(n-1)$-gaps of a polynomial $f$ of degree $m$ do \emph{not} approach infinity. Then the $\liminf$ of the smallest $(n-1)$-gap is finite, say $l$. We can write this as
		\[ \liminf_{i\to\infty} G_{n-1}\big[(1-D)^i f\big] = l \]
	where $G_n[f]$ is the size of the smallest $n$-gap of $f$. Choose $\e$ so that two (isolated) roots with separation less than $l+\e$ will have their separation increased by at least $3\e$. Choose $L$ large enough that
	\begin{enumerate}
		\item If an $(n-1)$-gap is at most $l+m+\e$ wide, and all roots outside the gap are at least $L$ away, then the size of the gap increases; and
		\item If an $(n-1)$-gap is at most $l+\e$ wide, and all roots outside the gap are at least $L$ away, then the outside roots' effect on the change in gap size is at most $\e$.
	\end{enumerate}
	By the assumption that the $n$-gaps approach infinity, there exists $N$ so that for all $i>N$
		\[ G_n\big[(1-D)^i f\big] > L + l + m + \e. \]
	By the assumption that the $\liminf$ of the smallest $(n-1)$-gap is $l$, there exist arbitrarily large $j$ such that 
		\[ l-\e < G_{n-1}\big[ (1-D)^j f\big] < l+\e. \]
	Choose such a $j$ which is greater than $N$. Due to the choice of $\e$ and $N$, we then have
		\[ G_{n-1}\big[ (1-D)^{j+1} f\big] > l+\e. \]
	For all further iterations, we have that an $(n-1)$-gap either increases, or if it is larger than $l+m+\e$, it may decrease. However, it may only decrease by at most $m$. Therefore the size of an $(n-1)$-gap will never drop below $l+\e$, contradicting that $l$ is the $\liminf$. It must then be that the $\liminf$ is infinite, so the size of the smallest $(n-1)$-gap approaches infinity.
\end{proof}

Lemmas \ref{lem:maxgapinf} and \ref{lem:gapinduction} together immediately give
\begin{theorem}
	If $f$ is any polynomial, the difference between any pair of roots of $(1-D)^n f$ approaches infinity as $n$ approaches infinity.
\end{theorem}

However, in a sense the roots tend to converge on their average, as given by the following theorem.
\begin{theorem}
	If $f$ is any polynomial, then for any $i$ the ratio of the $i$th root of $(1-D)^nf$ to the average root approaches $1$ as $n$ approaches infinity.
\end{theorem}
\begin{proof}
	Because the coefficients of a polynomial are the symmetric polynomials in its roots, given $f(x)=\sum a_i x^i$ with roots $\mu_1,\cdots,\mu_m$ and average root $\mu_{\avg}$ it follows that the polynomial
		\[ \sum_{i=0}^m \frac{a_i}{\mu_{\avg}^{m-i}}x^i \]
	has roots $\mu_i/\mu_{\avg}$. Therefore we want to show that as $n$ approaches infinity, the polynomial obtained by dividing the $i$th coefficient of $(1-D)^n f$ by the $(m-i)$th power of its average root approaches $(x-1)^m$.
	
	$1-D$ always increases the average root by 1, so
		\[ \mu_{\avg}^{(n)} = \mu_{\avg}+n. \]
	We now just need to calculate the coefficients $a_i^{(n)}$. It will ease the calculations if we first notice that the coefficients do not need to be calculated exactly: since the denominator will be degree $m-i$ in $n$ we only need to keep track of terms that are at least that big. We may also assume that $f$ is monic.
	
	Using these simplifying observations we will prove by induction on $i$ that
		\[ a_{i}^{(n)} = (-1)^{m-i}\binom{m}{i}n^{m-i} + \text{lower order terms,} \]
	so that the result will immediately follow.
	
	For $i=m$, the equation is trivial because we have assumed $f$ is monic:
		\[ a_m^{(n)} = 1. \]
	This provides the base case for our induction.
	
	Now suppose the equation holds for some $i$; we will show it also holds for $i-1$. We have
		\[ a_{i-1}^{(n)} = a_{i-1}^{(n-1)} - i a_i^{(n-1)} \]
	which by the inductive assumption is equal to
		\[ a_{i-1}^{(n-1)} - i (-1)^{m-i}\binom{m}{i}n^{m-i} + \text{lower order terms}. \]
	Repeating this $n-1$ times gives that
		\[ a_{i-1}^{(n)} = a_{i-1} - \sum_{j=1}^n i (-1)^{m-i} \binom{m}{i} j^{m-i} + \text{lower order terms} \]
		\[ = i (-1)^{m-i+1} \binom{m}{i} \sum_{j=1}^n j^{m-i} + \text{lower order terms.} \]
	The exact formula for this sum is
		\[ \sum_{j=1}^n j^{m-i} = \frac{1}{m-i+1}\sum_{k=0}^{m-i} \binom{m-i+1}{k}B_k n^{m-i+1-k} \]
	but again we are only interested in the largest degree term, where $k=0$:
		\[ \frac{1}{m-i+1}n^{m-i+1}. \]
	Therefore we now have
		\[ a_{i-1}^{(n)} = (-1)^{m-(i-1)} i \frac{m!}{i!(m-i)} \cdot \frac{1}{m-i+1} n^{m-i+1} = (-1)^{m-(i-1)} \binom{m}{i-1} n^{m-(i-1)} \]
	which is what we wanted.
\end{proof}

\begin{thebibliography}{9}
\bibitem{diffspacing}
 Farmer, D.W. and Rhoades, R.C.
 \emph{Differentiation Evens out Zero Spacings}.
 arXiv:math/0310252.

\end{thebibliography}

\end{document}

